Zcash/Snark/Soundness/Action/AdaptiveStatementInhabitant.lean
@@ -1,5 +1,5 @@
 import Zcash.Snark.Soundness.Action.AdaptiveStatementModel
-import Zcash.Circuits.Integration.PermutationColumns
+import Zcash.Snark.Soundness.Multiopen.PermutationColumns
 import Zcash.Snark.Soundness.AGM.ZeroFamily
 
 /-!
